\documentclass{article}
\usepackage[utf8]{inputenc}
\usepackage[T1]{fontenc}
\usepackage{geometry}
\usepackage{amsmath}
\usepackage{amsfonts}
\usepackage{amssymb}
\usepackage{enumitem}

\geometry{
 letterpaper,
 margin=1.5cm
}

\begin{document}

\begin{enumerate}[label=\bfseries\small 143.\arabic*, itemsep=3cm]
\large

\item $a(x+1) = 1$

\item $ax-4 = bx-2$

\item $ax+b^2 = a^2 - bx$

\item $3(2a-x) + ax = a^2 + 9$

\item $a(x+b) + x(b-a) = 2b(2a-x)$

\item $(x-a)^2 - (x+a)^2 = a(a-7x)$

\item $ax-a(a+b) = -x - (1+ab)$

\item $a^2(a-x) - b^2(x-b) = b^2(x-b)$

\item $(x+a)(x-b) - (x+b)(x-2a) = b(a-2) + 3a$

\item $x^2 + a^2 = (a+x)^2 - a(a-1)$

\item $m(n-x) - m(n-1) = m(mx-a)$

\item $x-a+2=2ax-3(a+x)-2(a-5)$

\item $a(x-a)-2bx=b(b-2a-x)$

\item $ax+bx=(x+a-b)^2-(x-2b)(x+2a)$

\item $x(a+b)-3-a(a-2)=2(x-1)-x(a-b)$

\item $(m+4x)(3m+x)=(2x-m)^2+m(15x-m)$

\item $a^2(a-x)-a^2(a+1)-b^2(b-x)-b(1-b^2)+a(1+a)=0$

\item $(ax-b)^2=(bx-a)(a+x)-x^2(b-a^2)+a^2+b(1-2b)$

\item $(x+b)^2-(x-a)^2-(a+b)^2=0$

\item $(x+m)^3-12m^3=-{(x-m)}^3+2x^3$


\end{enumerate}

\end{document}