\documentclass{article}
\usepackage[utf8]{inputenc}
\usepackage[T1]{fontenc}
\usepackage{geometry}
\usepackage{amsmath}
\usepackage{amsfonts}
\usepackage{amssymb}
\usepackage{enumitem}

\geometry{
 letterpaper,
 margin=1.5cm
}

\begin{document}

\begin{enumerate}[label=\bfseries\small 141.\arabic*, itemsep=4cm]
\large

\item $\dfrac{x}{6} + 5 = \dfrac{1}{3} - x$

\item $\dfrac{3x}{5} - \dfrac{2x}{3} + \dfrac{1}{5} = 0$

\item $\dfrac{1}{2x} + \dfrac{1}{4} - \dfrac{1}{10x} = \dfrac{1}{5}$

\item $\dfrac{x}{2} + 2 - \dfrac{x}{12} = \dfrac{x}{6} - \dfrac{5}{4}$

\item $\dfrac{3x}{4} - \dfrac{1}{5} + 2x = \dfrac{5}{4} - \dfrac{3x}{20}$

\item $\dfrac{2}{3x} - \dfrac{5}{x} = \dfrac{7}{10} - \dfrac{3}{2x} + 1$

\item $\dfrac{x-4}{3} - 5 = 0$

\item $x - \dfrac{x+2}{12} = \dfrac{5x}{2}$

\item $x - \dfrac{5x-1}{3} = 4x - \dfrac{3}{5}$

\item $10x - \dfrac{8x-3}{4} = 2(x-3)$

\item $\dfrac{x-2}{3} - \dfrac{x-3}{4} = \dfrac{x-4}{5}$

\item $\dfrac{x-1}{2} - \dfrac{x-2}{3} - \dfrac{x-3}{4} = -\dfrac{x-5}{5}$

\item $x - (5x-1) - \dfrac{7-5x}{10} = 1$

\item $2x - \dfrac{5x-6}{4} + \dfrac{1}{3}(x-5) = -5x$

\item $4 - \dfrac{10x+1}{6} = 4x - \dfrac{16x+3}{4}$

\item $\dfrac{1}{2}(x-1) - (x-3) = \dfrac{1}{3}(x+3) + \dfrac{1}{6}$

\item $\dfrac{6x+1}{3} - \dfrac{11x-2}{9} - \dfrac{1}{4}(5x-2) = \dfrac{5}{6}(6x+1)$

\item $\dfrac{4x+1}{3} = \dfrac{1}{3}(4x-1) - \dfrac{13+2x}{6} - \dfrac{1}{2}(x-3)$

\item $\dfrac{2}{5}(5x-1) + \dfrac{3}{10}(10x-3) = -\dfrac{1}{2}(x-2) - \dfrac{6}{5}$

\item $\dfrac{3x-1}{2} - \dfrac{5x+4}{3} - \dfrac{x+2}{8} = \dfrac{2x-3}{5} - \dfrac{1}{10}$

\item $\dfrac{7x-1}{3} - \dfrac{5-2x}{2x} = \dfrac{4x-3}{4} + \dfrac{1+4x^2}{3x}$

\item $\dfrac{2x+7}{3} - \dfrac{2(x^2-4)}{5x} - \dfrac{4x^2-6}{15x} = \dfrac{7x^2+6}{3x^2}$

\item $\dfrac{2}{3}\left(\dfrac{x+1}{5}\right) = \dfrac{3}{4}\left(\dfrac{x-6}{3}\right)$

\item $\dfrac{3}{5}\left(\dfrac{2x-1}{6}\right) - \dfrac{4}{3}\left(\dfrac{3x+2}{4}\right) - \dfrac{1}{5}\left(\dfrac{x-2}{3}\right) + \dfrac{1}{5} = 0$

\item $10 - \dfrac{3x+5}{6} = 3\dfrac{11}{12} - \dfrac{\dfrac{x}{2}}{4}$

\item $9x - 2 - 7x\left(\dfrac{1}{x}-\dfrac{1}{2}\right) = \dfrac{1+\dfrac{x}{2}}{2} + 2\dfrac{3}{4}$

\item $\dfrac{3x}{8} - \dfrac{7}{10} - \dfrac{12x - 5}{16} - \dfrac{2x - 3}{20} + \dfrac{4x + 9}{4} + \dfrac{7}{80} = 0$

\item $\dfrac{5x}{4} - \dfrac{3}{17}(x - 20) - (2x - 1) = \dfrac{x + 24}{34}$

\item $5 + \dfrac{x}{4} = \dfrac{1}{3} \left( 2 - \dfrac{x}{2} \right) - \dfrac{2}{3} + \dfrac{1}{4} \left( 10 - \dfrac{5x}{3} \right)$

\item $\dfrac{5(x + 2)}{12} + \dfrac{4}{9} - \dfrac{22 - x}{36} = 3x - 20 - \dfrac{8 - x}{12} - \dfrac{20 - 3x}{18}$

\item $\left( 3 - \dfrac{x}{2} \right) - \left( 1 - \dfrac{x}{3} \right) = 7 - \left( x - \dfrac{x}{2} \right)$

\item $(x + 3)(x - 3) - x^2 - \dfrac{5}{4} = \left( x - \dfrac{x}{5} \right) - \left( 3x - \dfrac{3}{4} \right)$

\item $2x - \left( 2x - \dfrac{3x - 1}{8} \right) = \dfrac{2}{3} \left( \dfrac{x + 2}{6} \right) - \dfrac{1}{4}$

\end{enumerate}

\end{document}