\documentclass{article}
\usepackage[utf8]{inputenc}
\usepackage[T1]{fontenc}
\usepackage{geometry}
\usepackage{amsmath}
\usepackage{amsfonts}
\usepackage{amssymb}
\usepackage{enumitem}

\geometry{
 letterpaper,
 margin=1.5cm
}

\begin{document}

\begin{enumerate}[label=\bfseries\small 142.\arabic*, itemsep=4cm]
\large

\item $\dfrac{3}{5} + \dfrac{3}{2x - 1} = 0$

\item $\dfrac{2}{4x - 1} = \dfrac{3}{4x + 1}$

\item $\dfrac{5}{x^2 - 1} = \dfrac{1}{x - 1}$

\item $\dfrac{3}{x + 1} - \dfrac{1}{x^2 - 1} = 0$

\item $\dfrac{5x + 8}{3x + 4} = \dfrac{5x + 2}{3x - 4}$

\item $\dfrac{10x^2 - 5x + 8}{5x^2 + 9x - 19} = 2$

\item $\dfrac{1}{3x-3} + \dfrac{1}{4x+4} = \dfrac{1}{12x-12}$

\item $\dfrac{x}{4} + \dfrac{x^2 - 8x}{4x-5} = \dfrac{7}{4}$

\item $\dfrac{2x-9}{10} + \dfrac{2x-3}{2x-1} = \dfrac{x}{5}$

\item $\dfrac{(3x-1)^2}{x-1} = \dfrac{18x-1}{2}$

\item $\dfrac{2x+7}{5x+2} - \dfrac{2x-1}{5x-4} = 0$

\item $\dfrac{(5x-2)(7x+3)}{7x(5x-1)} - 1 = 0$

\item $\dfrac{3}{x-4} = \dfrac{2}{x-3} + \dfrac{8}{x^2 - 7x + 12}$

\item $\dfrac{6x-1}{18} - \dfrac{3(x+2)}{5x-6} = \dfrac{1+3x}{9}$

\item $\dfrac{5}{1+x} - \dfrac{3}{1-x} - \dfrac{6}{1-x^2} = 0$

\item $\dfrac{1+2x}{1+3x} - \dfrac{1-2x}{1-3x} = -\dfrac{3x-14}{1-9x^2}$

\item $\dfrac{3x-1}{x^2+7x+12} = \dfrac{1}{2x+6} + \dfrac{7}{6x+24}$

\item $\dfrac{1}{(x-1)^2} - \dfrac{3}{2x-2} = \dfrac{3}{2x+2}$

\item $\dfrac{5x+13}{15} - \dfrac{4x+5}{5x-15} = \dfrac{x}{3}$

\item $\dfrac{2x-1}{2x+1} - \dfrac{x-4}{3x-2} = \dfrac{2}{3}$

\item $\dfrac{4x+3}{2x-5} - \dfrac{3x+8}{3x-7} = 1$

\item $\dfrac{10x-7}{15x+3} = \dfrac{3x+8}{12} - \dfrac{5x^2-4}{20x+4}$

\item $\dfrac{4x-1}{5} + \dfrac{x-2}{2x-7} = \dfrac{8x-3}{10} - 1\dfrac{3}{10}$

\item $\dfrac{1}{x-1} - \dfrac{2}{x-2} = \dfrac{3}{2x-2} - \dfrac{2\dfrac{1}{3}}{2x-4}$

\item $\dfrac{1}{x+3} - \dfrac{2}{5x-20} = \dfrac{1\dfrac{1}{2}}{3x-12} - \dfrac{2}{x+3}$

\item $\dfrac{1}{6-2x} - \dfrac{4}{5-5x} = \dfrac{10}{12-4x} - \dfrac{3}{10-10x}$

\item $\dfrac{2}{3} - \dfrac{6x^2}{9x^2-1} = \dfrac{2}{3x-1}$

\item $\dfrac{5x^2 - 27x}{5x + 3} - \dfrac{1}{x} = x - 6$

\item $\dfrac{4x + 1}{4x - 1} - \dfrac{6}{16x^2 - 1} = \dfrac{4x - 1}{4x + 1}$

\item $3 \left( \dfrac{x - 1}{x + 1} \right) + 2 \left( \dfrac{x + 1}{x - 4} \right) = \dfrac{5x(x - 1)}{x^2 - 3x - 4}$

\item $2 \left( \dfrac{x + 2}{x - 2} \right) - 3 \left( \dfrac{x - 2}{2x + 3} \right) = \dfrac{x^2 + 78}{2x^2 - x - 6}$

\item $\dfrac{1}{x^2 + 3x - 28} - \dfrac{1}{x^2 + 12x + 35} = \dfrac{3}{x^2 + x - 20}$

\item $\dfrac{x - 2}{x^2 + 8x + 7} = \dfrac{2x - 5}{x^2 - 49} - \dfrac{x - 2}{x^2 - 6x - 7}$

\item $\dfrac{4x + 5}{15x^2 + 7x - 2} - \dfrac{2x + 3}{12x^2 - 7x - 10} - \dfrac{2x - 5}{20x^2 - 29x + 5} = 0$

\item $\dfrac{7}{2x + 1} - \dfrac{3}{x + 4} = \dfrac{2}{x + 1} - \dfrac{3(x + 1)}{2x^2 + 9x + 4}$

\item $\dfrac{(x + 3)^2}{(x - 3)^2} = \dfrac{x - 1}{x + 1} + \dfrac{2(7x + 1)}{x^2 - 2x - 3}$

\item $\dfrac{x - 4}{x + 5} - \dfrac{x + 1}{x - 2} = -\dfrac{12(x + 3)}{(x + 5)^2}$

\item $\dfrac{x - 3}{x - 4} - \dfrac{x - 2}{x - 3} = \dfrac{x + 2}{x + 1} - \dfrac{x + 3}{x + 2}$

\item $\dfrac{x + 6}{x + 2} - \dfrac{x + 1}{x - 3} = \dfrac{x - 5}{x - 1} - \dfrac{x}{x + 4}$


\end{enumerate}

\end{document}