\documentclass{article}
\usepackage[utf8]{inputenc}
\usepackage[T1]{fontenc}
\usepackage{geometry}
\usepackage{amsmath}
\usepackage{amsfonts}
\usepackage{amssymb}
\usepackage{enumitem}

\geometry{
 letterpaper,
 margin=1.5cm
}

\begin{document}

\begin{enumerate}[label=\bfseries\small 144.\arabic*, itemsep=3cm]
\large

\item $\dfrac{m}{x} - \dfrac{1}{m} = \dfrac{2}{m}$

\item $\dfrac{a}{x} + \dfrac{b}{2} = \dfrac{4a}{x}$

\item $\dfrac{x}{2a} - \dfrac{1-x}{a^2} = \dfrac{1}{2a}$

\item $\dfrac{m}{x} + \dfrac{n}{m} = \dfrac{n}{x} + 1$

\item $\dfrac{a-1}{a} + \dfrac{1}{2} = \dfrac{3a-2}{x}$

\item $\dfrac{a-x}{a} - \dfrac{b-x}{b} = \dfrac{2(a-b)}{ab}$

\item $\dfrac{x - 3a}{a^2} - \dfrac{2a - x}{ab} = -\dfrac{1}{a}$

\item $\dfrac{x + m}{m} - \dfrac{x + n}{n} = \dfrac{m^2 + n^2}{mn} - 2$

\item $\dfrac{x - b}{a} = 2 - \dfrac{x - a}{b}$

\item $\dfrac{4x}{2a + b} - 3 = -\dfrac{3}{2}$

\item $\dfrac{2a + 3x}{x + a} = \dfrac{2(6x - a)}{4x + a}$

\item $\dfrac{2(x - c)}{4x - b} = \dfrac{2x + c}{4(x - b)}$

\item $\dfrac{1}{n} - \dfrac{m}{x} = \dfrac{1}{mn} - \dfrac{1}{x}$

\item $\dfrac{(x-2b)(2x+a)}{(x-a)(a-2b+x)} = 2$

\item $\dfrac{x+m}{x-n} = \dfrac{n+x}{m+x}$

\item $\dfrac{x(2x+3b)(x+b)}{x+3b} = 2x^2 - bx + b^2$

\item $\dfrac{3}{4}\left(\dfrac{x}{b} + \dfrac{x}{a}\right) = \dfrac{1}{3}\left(\dfrac{x}{b} - \dfrac{x}{a}\right) + \dfrac{5a + 13b}{12a}$

\item $\dfrac{x+a}{3} = \dfrac{(x-b)^2}{3x-a} + \dfrac{3ab-3b^2}{9x-3a}$

\item $\dfrac{5x+a}{3x+b} = \dfrac{5x-b}{3x-a}$

\item $\dfrac{x+a}{x-a} - \dfrac{x-a}{x+a} = \dfrac{a(2x+ab)}{x^2-a^2}$

\item $\dfrac{2x - 3a}{x + 4a} - 2 = \dfrac{11a}{x^2 - 16a^2}$

\item $\dfrac{1}{x + a} + \dfrac{x^2}{a^2 + ax} = \dfrac{x + a}{a}$

\item $\dfrac{2(a + x)}{b} - \dfrac{3(b + x)}{a} = \dfrac{6(a^2 - 2b^2)}{ab}$

\item $m(n - x) - (m - n)(m + x) = n^2 - \dfrac{1}{n}(2mn^2 - 3m^2n)$

\end{enumerate}

\end{document}