\documentclass{article}
\usepackage[utf8]{inputenc}
\usepackage[T1]{fontenc}
\usepackage{geometry}
\usepackage{amsmath}
\usepackage{amsfonts}
\usepackage{amssymb}
\usepackage{enumitem}

\geometry{
 letterpaper,
 margin=1.5cm
}

\begin{document}

\begin{enumerate}[label=\bfseries\small 139.\arabic*, itemsep=3cm]
\large


\item $\dfrac{x-2}{x+3}$ para $x = 2$

\item $\dfrac{x-2}{x-3}$ para $x = 3$

\item $\dfrac{x^2 - a^2}{x^2 + a^2}$ para $x = a$

\item $\dfrac{x^2 + y^2}{x^2 - y^2}$ para $x = y$

\item $\dfrac{x - 1}{\dfrac{3}{x - 2}}$ para $x = 2$ 

\item $\dfrac{x^2 - 9}{x^2 + x - 12}$ para $x = 3$

\item $\dfrac{a^2 - a - 6}{a^2 + 2a - 15}$ para $a = 3$

\item $\dfrac{x^2 - 7x + 10}{x^3 - 2x^2 - x + 2}$ para $x = 2$

\item $\dfrac{x^2 - 2x + 1}{x^3 - 2x^2 - x + 2}$ para $x = 1$

\item $\dfrac{a^3 - 8}{a^2 + 11a - 26}$ para $a = 2$

\item $\dfrac{x^2 - 7x + 6}{x^2 - 2x + 1}$ para $x = 1$

\item $\dfrac{x^3 - 3x - 2}{x^3 - 7x + 6}$ para $x = 2$

\item $\dfrac{x^2 - 16}{x^3 - 4x^2 - x + 4}$ para $x = 4$

\item $\dfrac{4x^2 - 4x + 1}{4x^2 + 8x - 5}$ para $x = \dfrac{1}{2}$

\item $\dfrac{8x^2 - 6x + 1}{4x^3 + 12x^2 - 15x + 4}$ para $x = \dfrac{1}{2}$

\item $\dfrac{x^3 - 9x + 10}{x^4 - x^3 - 11x^2 + 9x + 18}$ para $x = 2$

\item $\dfrac{x^3 - a^3}{x - a}$ para $x = a$

\item $\dfrac{a^2 - 2a + b^2}{a^2 - ab}$ para $b = a$

\item $\dfrac{x^2 - y^2}{xy - y^2}$ para $y = x$

\item $\dfrac{x^3 - a^3}{a^2 x - a^3}$ para $x = a$

\item $\dfrac{x^3 - 3x + 2}{2x^3 - 6x^2 + 6x - 2}$ para $x = 1$

\item $\dfrac{x^4 - x^3 - 7x^2 + x + 6}{x^4 - 3x^3 - 3x^2 + 11x - 6}$ para $x = 3$

\item $\dfrac{3x^3 - 5x^2 - 4x + 4}{x^4 + 2x^3 - 3x^2 + 8x - 4}$ para $x = 2$

\item $\dfrac{x^2 - 5x + 4}{x^4 - 2x^3 - 9x^2 + 2x + 8}$ para $x = 1$

\item $\dfrac{x^5 - 4x^3 + 8x^2 - 32}{x^5 - 3x^3 + 10x^2 - 4x - 40}$ para $x = 2$

\item $\dfrac{8x^2 + 6x - 9}{12x^2 - 13x + 3}$ para $x = \dfrac{3}{4}$

\item $\dfrac{x^3 + 6x^2 + 12x + 8}{x^4 - 8x^2 + 16}$ para $x = -2$

\item $\dfrac{9x^3 + 3x^2 + 3x + 1}{27x^3 + 1}$ para $x = -\dfrac{1}{3}$

\item $\dfrac{1}{x - 1} - \dfrac{3}{x^3 - 1}$ para $x = 1$

\item $(x^2 + 3x - 10) \left( 1 + \dfrac{1}{x - 2} \right)$ para $x = 2$


\end{enumerate}

\end{document}